rename Mod2STS.v to Mod2ITree.v

imp_system/imp/Imp.v
@@ -556,7 +556,7 @@ Section Interp.
       end.
 
   Definition interp_ImpState {eff} `{coreE -< eff}: itree (ImpState +' eff) ~> stateT lenv (itree eff) :=
-    State.interp_state (case_ handle_ImpState Mod2STS.pure_state).
+    State.interp_state (case_ handle_ImpState Mod2ITree.pure_state).
 
   (* Definition interp_imp ge le (itr : itree effs val) := *)
   (*   interp_ImpState (interp_GlobEnv ge itr) le. *)
